Iris/Iris/BI/Lib.lean
@@ -7,6 +7,7 @@ public import Iris.BI.Lib.Fixpoint
 public import Iris.BI.Lib.FixpointBanach
 public import Iris.BI.Lib.Fractional
 public import Iris.BI.Lib.GenHeap
+public import Iris.BI.Lib.InvHeap
 public import Iris.BI.Lib.Laterable
 public import Iris.BI.Lib.MonoNat
 public import Iris.BI.Lib.ProphMap
